start linearizing Variables

Impl/StateBCImpl.i.dfy
@@ -1,5 +1,5 @@
 include "../lib/Base/DebugAccumulator.i.dfy"
-include "../lib/DataStructures/LruImpl.i.dfy"
+include "../lib/DataStructures/LinearLru.i.dfy"
 include "IndirectionTable.i.dfy"
 include "StateBCModel.i.dfy"
 include "StateSectorImpl.i.dfy"
@@ -13,221 +13,184 @@ module StateBCImpl {
   import opened NativeTypes
   import opened StateSectorImpl
   import opened CacheImpl
-  import IndirectionTable
+  import IT = IndirectionTable
   import opened Bounds
+  import opened LinearOption
 
   import BitmapImpl
   import DebugAccumulator
   import DiskLayout
   import BT = PivotBetreeSpec`Internal
   import BC = BlockCache
-  import LruImpl
+  import LinearLru
   import BlockAllocatorImpl
   import D = AsyncDisk
   import SBCM = StateBCModel
+
 
   type ImplVariables = Variables
   type Reference = BT.G.Reference
 
   // TODO rename to like... BlockCache variables or smthn
-  class Variables {
-    var loading: bool;
-    var ready: bool;
+  linear datatype Variables = Variables(
+    loading: bool,
+    ready: bool,
 
     // Ready
-    var persistentIndirectionTable: MutIndirectionTable;
-    var frozenIndirectionTable: MutIndirectionTableNullable;
-    var ephemeralIndirectionTable: MutIndirectionTable;
-    var persistentIndirectionTableLoc: DiskLayout.Location;
-    var frozenIndirectionTableLoc: Option<DiskLayout.Location>;
-    var outstandingIndirectionTableWrite: Option<BC.ReqId>;
-    var outstandingBlockWrites: map<D.ReqId, BC.OutstandingWrite>;
-    var outstandingBlockReads: map<D.ReqId, BC.OutstandingRead>;
-    var cache: MutCache;
-    var lru: LruImpl.LruImplQueue;
-    var blockAllocator: BlockAllocatorImpl.BlockAllocator;
+    linear persistentIndirectionTable: IT.IndirectionTable,
+    linear frozenIndirectionTable: lOption<IT.IndirectionTable>,
+    linear ephemeralIndirectionTable: IT.IndirectionTable,
+    persistentIndirectionTableLoc: DiskLayout.Location,
+    frozenIndirectionTableLoc: Option<DiskLayout.Location>,
+    outstandingIndirectionTableWrite: Option<BC.ReqId>,
+    outstandingBlockWrites: map<D.ReqId, BC.OutstandingWrite>,
+    outstandingBlockReads: map<D.ReqId, BC.OutstandingRead>,
+    linear cache: LMutCache,
+    linear lru: LinearLru.LinearLru,
+    linear blockAllocator: BlockAllocatorImpl.BlockAllocator,
 
     // Loading
-    var indirectionTableLoc: DiskLayout.Location;
-    var indirectionTableRead: Option<BC.ReqId>;
-
+    indirectionTableLoc: DiskLayout.Location,
+    indirectionTableRead: Option<BC.ReqId>
+    
     // Unready
     // no fields
+  )
+  {
+      // method DebugAccumulate()
+      // returns (acc:DebugAccumulator.DebugAccumulator)
+      // requires false
+      // {
+      //   acc := DebugAccumulator.EmptyAccumulator();
+      //   //var r := new DebugAccumulator.AccRec(syncReqs.Count, "SyncReqStatus");
+      //   //acc := DebugAccumulator.AccPut(acc, "syncReqs", r);
+      //   var i := DebugAccumulator.EmptyAccumulator();
+      //   if persistentIndirectionTable != null {
+      //     i := persistentIndirectionTable.DebugAccumulate();
+      //   }
+      //   var a := new DebugAccumulator.AccRec.Index(i);
+      //   acc := DebugAccumulator.AccPut(acc, "persistentIndirectionTable", a);
+      //   i := DebugAccumulator.EmptyAccumulator();
+      //   if frozenIndirectionTable != null {
+      //     i := frozenIndirectionTable.DebugAccumulate();
+      //   }
+      //   a := new DebugAccumulator.AccRec.Index(i);
+      //   acc := DebugAccumulator.AccPut(acc, "frozenIndirectionTable", a);
+      //   i := DebugAccumulator.EmptyAccumulator();
+      //   if ephemeralIndirectionTable != null {
+      //     i := ephemeralIndirectionTable.DebugAccumulate();
+      //   }
+      //   a := new DebugAccumulator.AccRec.Index(i);
+      //   acc := DebugAccumulator.AccPut(acc, "ephemeralIndirectionTable", a);
+      //   //r := new DebugAccumulator.AccRec(if outstandingIndirectionTableWrite.Some? then 1 else 0, "ReqId");
+      //   //acc := DebugAccumulator.AccPut(acc, "outstandingIndirectionTableWrite", r);
+      //   //r := new DebugAccumulator.AccRec(|outstandingBlockWrites| as uint64, "OutstandingWrites");
+      //   //acc := DebugAccumulator.AccPut(acc, "outstandingBlockWrites", r);
+      //   //r := new DebugAccumulator.AccRec(|outstandingBlockReads| as uint64, "OutstandingReads");
+      //   //acc := DebugAccumulator.AccPut(acc, "outstandingBlockReads", r);
+      //   i := cache.DebugAccumulate();
+      //   a := new DebugAccumulator.AccRec.Index(i);
+      //   acc := DebugAccumulator.AccPut(acc, "cache", a);
+      //   i := lru.DebugAccumulate();
+      //   a := new DebugAccumulator.AccRec.Index(i);
+      //   acc := DebugAccumulator.AccPut(acc, "lru", a);
+      //   i := blockAllocator.DebugAccumulate();
+      //   a := new DebugAccumulator.AccRec.Index(i);
+      //   acc := DebugAccumulator.AccPut(acc, "blockAllocator", a);
+      // }
 
-    // method DebugAccumulate()
-    // returns (acc:DebugAccumulator.DebugAccumulator)
-    // requires false
+      predicate W()
+      {
+        && persistentIndirectionTable.Inv()
+        && (frozenIndirectionTable.lSome? ==> frozenIndirectionTable.value.Inv())
+        && ephemeralIndirectionTable.Inv()
+        && lru.Inv()
+        && cache.Inv()
+        && blockAllocator.Inv()
+      }
+
+      function I() : SBCM.BCVariables
+      requires W()
+      {
+        if ready then (
+          SBCM.Ready(
+            persistentIndirectionTable,
+            if frozenIndirectionTable.lSome? then Some(frozenIndirectionTable.value) else None,
+            ephemeralIndirectionTable,
+            persistentIndirectionTableLoc,
+            frozenIndirectionTableLoc,
+            outstandingIndirectionTableWrite,
+            outstandingBlockWrites,
+            outstandingBlockReads,
+            cache.I(),
+            lru.Queue(),
+            blockAllocator.I())
+        ) else if loading then (
+          SBCM.LoadingIndirectionTable(
+            indirectionTableLoc,
+            indirectionTableRead)
+        ) else (
+          SBCM.Unready
+        )
+      }
+
+      predicate WF()
+      {
+        && W()
+        && SBCM.WFBCVars(I())
+      }
+
+      static method Constructor() returns (linear v: Variables)
+      ensures !v.ready
+      ensures !v.loading
+      ensures v.WF()
+      {
+        linear var lru := LinearLru.LinearLru.Alloc();
+        // Unused for the `ready = false` state but we need to initialize them.
+        // (could make them nullable instead).
+        linear var ephemeralIndirectionTable := IT.IndirectionTable.AllocEmpty();
+        linear var persistentIndirectionTable := IT.IndirectionTable.AllocEmpty();
+        linear var cache := LMutCache.NewCache();
+
+        linear var bm := BitmapImpl.Bitmap.Constructor(NumBlocksUint64());
+        linear var blockAllocator := BlockAllocatorImpl.BlockAllocator.Constructor(bm);
+
+        v := Variables(
+          false,
+          false,
+          persistentIndirectionTable,
+          lNone,
+          ephemeralIndirectionTable,
+          DiskLayout.Location(0, 0),
+          None,
+          None,
+          map[],
+          map[],
+          cache,
+          lru,
+          blockAllocator,
+          DiskLayout.Location(0, 0),
+          None);
+      }
+
+      predicate Inv()
+      {
+        && W()
+        && SBCM.BCInv(I())
+      }
+
+    // twostate predicate WellUpdated(s: Variables)
     // {
-    //   acc := DebugAccumulator.EmptyAccumulator();
-    //   //var r := new DebugAccumulator.AccRec(syncReqs.Count, "SyncReqStatus");
-    //   //acc := DebugAccumulator.AccPut(acc, "syncReqs", r);
-    //   var i := DebugAccumulator.EmptyAccumulator();
-    //   if persistentIndirectionTable != null {
-    //     i := persistentIndirectionTable.DebugAccumulate();
-    //   }
-    //   var a := new DebugAccumulator.AccRec.Index(i);
-    //   acc := DebugAccumulator.AccPut(acc, "persistentIndirectionTable", a);
-    //   i := DebugAccumulator.EmptyAccumulator();
-    //   if frozenIndirectionTable != null {
-    //     i := frozenIndirectionTable.DebugAccumulate();
-    //   }
-    //   a := new DebugAccumulator.AccRec.Index(i);
-    //   acc := DebugAccumulator.AccPut(acc, "frozenIndirectionTable", a);
-    //   i := DebugAccumulator.EmptyAccumulator();
-    //   if ephemeralIndirectionTable != null {
-    //     i := ephemeralIndirectionTable.DebugAccumulate();
-    //   }
-    //   a := new DebugAccumulator.AccRec.Index(i);
-    //   acc := DebugAccumulator.AccPut(acc, "ephemeralIndirectionTable", a);
-    //   //r := new DebugAccumulator.AccRec(if outstandingIndirectionTableWrite.Some? then 1 else 0, "ReqId");
-    //   //acc := DebugAccumulator.AccPut(acc, "outstandingIndirectionTableWrite", r);
-    //   //r := new DebugAccumulator.AccRec(|outstandingBlockWrites| as uint64, "OutstandingWrites");
-    //   //acc := DebugAccumulator.AccPut(acc, "outstandingBlockWrites", r);
-    //   //r := new DebugAccumulator.AccRec(|outstandingBlockReads| as uint64, "OutstandingReads");
-    //   //acc := DebugAccumulator.AccPut(acc, "outstandingBlockReads", r);
-    //   i := cache.DebugAccumulate();
-    //   a := new DebugAccumulator.AccRec.Index(i);
-    //   acc := DebugAccumulator.AccPut(acc, "cache", a);
-    //   i := lru.DebugAccumulate();
-    //   a := new DebugAccumulator.AccRec.Index(i);
-    //   acc := DebugAccumulator.AccPut(acc, "lru", a);
-    //   i := blockAllocator.DebugAccumulate();
-    //   a := new DebugAccumulator.AccRec.Index(i);
-    //   acc := DebugAccumulator.AccPut(acc, "blockAllocator", a);
+    //   && s.W()
+    //   && (forall o | o in s.Repr() :: o in old(s.Repr()) || fresh(o))
     // }
 
-    function Repr() : set<object>
-    reads this, persistentIndirectionTable, ephemeralIndirectionTable,
-        frozenIndirectionTable, lru, cache, blockAllocator
+    shared function method TotalCacheSize() : (res : uint64)
+    requires cache.Inv()
+    requires |cache.I()| + |outstandingBlockReads| < 0x1_0000_0000_0000_0000
     {
-      {this} +
-      persistentIndirectionTable.Repr +
-      ephemeralIndirectionTable.Repr +
-      (if frozenIndirectionTable != null then frozenIndirectionTable.Repr else {}) +
-      lru.Repr +
-      cache.Repr +
-      blockAllocator.Repr
+      // cache.Count() + (|outstandingBlockReads| as uint64)
+      CacheImpl.CacheCount(cache) + (|outstandingBlockReads| as uint64)
     }
-
-    predicate ReprInv()
-    reads this, persistentIndirectionTable, ephemeralIndirectionTable,
-        frozenIndirectionTable, lru, cache, blockAllocator
-    reads Repr()
-    {
-        // NOALIAS statically enforced no-aliasing would probably help here
-        && persistentIndirectionTable.Repr !! ephemeralIndirectionTable.Repr !! lru.Repr !! cache.Repr !! blockAllocator.Repr
-        && (frozenIndirectionTable != null ==>
-            && frozenIndirectionTable.Repr !! persistentIndirectionTable.Repr
-            && frozenIndirectionTable.Repr !! ephemeralIndirectionTable.Repr
-            && frozenIndirectionTable.Repr !! lru.Repr
-            && frozenIndirectionTable.Repr !! cache.Repr
-            && frozenIndirectionTable.Repr !! blockAllocator.Repr
-        )
-
-        && this !in ephemeralIndirectionTable.Repr
-        && this !in persistentIndirectionTable.Repr
-        && (frozenIndirectionTable != null ==> this !in frozenIndirectionTable.Repr)
-        && this !in lru.Repr
-        && this !in cache.Repr
-        && this !in blockAllocator.Repr
-    }
-
-    predicate W()
-    reads this, persistentIndirectionTable, ephemeralIndirectionTable,
-        frozenIndirectionTable, lru, cache, blockAllocator
-    reads Repr()
-    {
-      && ReprInv()
-      && persistentIndirectionTable.Inv()
-      && (frozenIndirectionTable != null ==> frozenIndirectionTable.Inv())
-      && ephemeralIndirectionTable.Inv()
-      && lru.Inv()
-      && cache.Inv()
-      && blockAllocator.Inv()
-    }
-
-    function I() : SBCM.BCVariables
-    reads this, persistentIndirectionTable, ephemeralIndirectionTable,
-        frozenIndirectionTable, lru, cache, blockAllocator
-    reads Repr()
-    requires W()
-    {
-      if ready then (
-        SBCM.Ready(
-          persistentIndirectionTable.ReadWithInv(),
-          if frozenIndirectionTable != null then Some(frozenIndirectionTable.ReadWithInv()) else None,
-          ephemeralIndirectionTable.ReadWithInv(),
-          persistentIndirectionTableLoc,
-          frozenIndirectionTableLoc,
-          outstandingIndirectionTableWrite,
-          outstandingBlockWrites,
-          outstandingBlockReads,
-          cache.I(),
-          lru.Queue,
-          blockAllocator.I())
-      ) else if loading then (
-        SBCM.LoadingIndirectionTable(
-          indirectionTableLoc,
-          indirectionTableRead)
-      ) else (
-        SBCM.Unready
-      )
-    }
-
-    predicate WF()
-    reads this, persistentIndirectionTable, ephemeralIndirectionTable,
-        frozenIndirectionTable, lru, cache, blockAllocator
-    reads Repr()
-    {
-      && W()
-      && SBCM.WFBCVars(I())
-    }
-
-    constructor()
-    ensures !ready
-    ensures !loading
-    ensures WF()
-    ensures fresh(Repr())
-    {
-      ready := false;
-      loading := false;
-
-      // Unused for the `ready = false` state but we need to initialize them.
-      // (could make them nullable instead).
-      lru := new LruImpl.LruImplQueue();
-      ephemeralIndirectionTable := new MutIndirectionTable.Empty();
-      persistentIndirectionTable := new MutIndirectionTable.Empty();
-      frozenIndirectionTable := null;
-      cache := new MutCache();
-
-      var bm := new BitmapImpl.Bitmap(NumBlocksUint64());
-      blockAllocator := new BlockAllocatorImpl.BlockAllocator(bm);
-    }
-  }
-
-  predicate Inv(s: Variables)
-  reads s, s.persistentIndirectionTable, s.ephemeralIndirectionTable,
-        s.frozenIndirectionTable, s.lru, s.cache, s.blockAllocator
-  reads s.Repr()
-  {
-    && s.W()
-    && SBCM.BCInv(s.I())
-  }
-
-  twostate predicate WellUpdated(s: Variables)
-  reads s, s.persistentIndirectionTable, s.ephemeralIndirectionTable,
-      s.frozenIndirectionTable, s.lru, s.cache, s.blockAllocator
-  reads s.Repr()
-  {
-    && s.W()
-    && (forall o | o in s.Repr() :: o in old(s.Repr()) || fresh(o))
-  }
-
-  function method TotalCacheSize(s: ImplVariables) : (res : uint64)
-  reads s, s.cache, s.cache.Repr
-  requires s.cache.Inv()
-  requires |s.cache.I()| + |s.outstandingBlockReads| < 0x1_0000_0000_0000_0000
-  {
-    s.cache.Count() + (|s.outstandingBlockReads| as uint64)
   }
 }
